src/Dafny/examples/fs/mem_dirent.dfy
@@ -1,5 +1,6 @@
 include "dirent.dfy"
 include "paths.dfy"
+include "cursor.dfy"
 
 module MemDirEnts
 {
@@ -90,11 +91,13 @@ module MemDirEntries
   import opened Machine
   import opened ByteSlice
   import opened FsKinds
+  import opened JrnlSpec
   import IntEncoding
 
   import opened MemDirEnts
   import opened DirEntries
   import opened Paths
+  import opened FileCursor
 
   predicate dir_off?(k: uint64)
   {
@@ -104,12 +107,6 @@ module MemDirEntries
   function dirent_off(k: nat): nat
   {
     k * dirent_sz
-  }
-
-  function dirent_off_u64(k: uint64): uint64
-    requires dir_off?(k)
-  {
-    k * dirent_sz_u64
   }
 
   function path_ub(k: nat): nat
@@ -191,22 +188,29 @@ module MemDirEntries
   class MemDirents
   {
     ghost var val: Dirents
-    const bs: Bytes
+    const file: Cursor
 
-    ghost const Repr: set<object> := {this, bs}
+    function Repr(): set<object>
+      reads this.file
+    {
+        {this} + file.Repr()
+    }
 
     predicate {:opaque} ValidCore()
-      reads Repr
+      requires file.Valid()
+      reads this, file.Repr()
     {
-      && bs.data == val.enc()
-      && |bs.data| == 4096
+      && file.contents() == val.enc()
     }
 
     predicate Valid()
-      reads Repr
+      reads Repr()
     {
+      && file.Valid()
       && ValidCore()
-      && |val.s| == dir_sz
+        // arbitrary limit to prevent integer overflow
+      && |val.s| <= 1024
+      && |val.s| % 64 == 0
     }
 
     function dir(): Directory
@@ -215,56 +219,128 @@ module MemDirEntries
       val.dir
     }
 
-    constructor(bs: Bytes, ghost dents: Dirents)
-      requires bs.data == dents.enc()
+    constructor(file: Cursor, ghost dents: Dirents)
+      requires file.Valid()
+      requires file.contents() == dents.enc()
       requires |dents.s| == dir_sz
       ensures Valid()
       ensures val == dents
       // for framing
-      ensures this.bs == bs
+      ensures this.file == file
     {
-      this.bs := bs;
+      this.file := file;
       this.val := dents;
       new;
       reveal ValidCore();
     }
 
-    method encode() returns (bs': Bytes)
-      requires Valid()
-      ensures bs' == bs
-      ensures bs'.data == val.enc()
+    static function dir_blk(k: nat): nat
     {
-      reveal ValidCore();
-      bs' := bs;
+        k / 64 * 64
     }
 
-    method get_ino(k: uint64) returns (ino: Ino)
+    // offset of a whole-file offset within one paged-in block in the cursor
+    static function dir_blk_off(k: nat): nat
+    {
+        k % 64
+    }
+
+    predicate at_dir_off(k: nat)
+      reads this, file
+    {
+      && file.off as nat < |val.s|
+      && file.off as nat == dir_blk(k)
+      && file.bs != null
+    }
+
+    predicate has_jrnl(txn: Txn)
+      reads file.fs.Repr
+    {
+      file.fs.has_jrnl(txn)
+    }
+
+    method loadDirOff(txn: Txn, k: uint64)
+      modifies file
+      requires Valid() ensures Valid()
+      requires has_jrnl(txn)
+      requires k as nat < |val.s|
+      ensures at_dir_off(k as nat)
+    {
+      reveal ValidCore();
+      file.advanceTo(txn, k / 64 * 64);
+    }
+
+    lemma file_data(k: nat)
       requires Valid()
-      requires dir_off?(k)
+      requires at_dir_off(k)
+      ensures file.has_data(val.enc()[dir_blk(k) .. dir_blk(k) + 4096])
+    {
+      reveal ValidCore();
+      file.data_ok();
+    }
+
+    lemma file_bs_size()
+      requires file.Valid()
+      requires file.bs != null
+      ensures |file.bs.data| == 4096
+    {
+      reveal file.ValidBytes();
+    }
+
+    // give the caller the right double-subslice fact
+    lemma file_subslice(k: nat, start: nat, end: nat)
+      requires Valid()
+      requires at_dir_off(k)
+      requires start <= end <= 4096
+      ensures |file.bs.data| == 4096
+      ensures dir_blk(k) + end <= |file.contents()|
+      ensures file.bs.data[start..end] == file.contents()[dir_blk(k) + start .. dir_blk(k) + end]
+    {
+      file.data_ok();
+      C.double_subslice_auto(file.fs.data[file.ino]);
+    }
+
+    method get_ino(txn: Txn, k: uint64) returns (ino: Ino)
+      modifies file
+      requires Valid() ensures Valid()
+      requires has_jrnl(txn)
+      requires k as nat < |val.s|
       ensures ino == val.s[k].ino
     {
       reveal ValidCore();
+      loadDirOff(txn, k);
+      var off: uint64 := (k%64) * dirent_sz_u64 + path_len_u64;
+      file_subslice(k as nat, off as nat, off as nat + 8);
       // we'll prove it's an Ino later, for now it's just a uint64
-      var ino': uint64 := IntEncoding.UInt64Get(bs, k*dirent_sz_u64 + path_len_u64);
-      seq_data_one_ino(bs.data, val, k as nat);
+      var ino': uint64 := IntEncoding.UInt64Get(file.bs, off);
+      seq_data_one_ino(file.contents(), val, k as nat);
       ino := ino';
     }
 
-    method get_name(k: uint64) returns (name: Bytes)
-      requires Valid()
-      requires dir_off?(k)
-      ensures fresh(name) && name.Valid() && |name.data| == path_len
+    method get_name(txn: Txn, k: uint64) returns (name: Bytes)
+      modifies file
+      requires Valid() ensures Valid()
+      requires has_jrnl(txn)
+      requires k as nat < |val.s|
+      // since file.bs could also change, need to promise that it doesn't change
+      // to become name
+      ensures name != file.bs && fresh(name) && |name.data| == path_len
       ensures encode_pathc(val.s[k].name) == name.data
     {
       reveal ValidCore();
+      loadDirOff(txn, k);
       name := NewBytes(path_len_u64);
-      name.CopyFrom(bs, k*dirent_sz_u64, path_len_u64);
-      seq_data_one_name(bs.data, val, k as nat);
+      var start := (k%64) * dirent_sz_u64;
+      file_subslice(k as nat, start as nat, start as nat + path_len);
+      name.CopyFrom(file.bs, start, path_len_u64);
+      seq_data_one_name(file.contents(), val, k as nat);
     }
 
-    method get_dirent(k: uint64) returns (r:Option<MemDirEnt>)
-      requires Valid()
-      requires dir_off?(k)
+    method get_dirent(txn: Txn, k: uint64) returns (r:Option<MemDirEnt>)
+      modifies file
+      requires Valid() ensures Valid()
+      requires has_jrnl(txn)
+      requires k as nat < |val.s|
       ensures r.None? ==> !val.s[k].used()
       ensures r.Some? ==>
       && val.s[k].used()
@@ -272,38 +348,42 @@ module MemDirEntries
       && r.x.Valid()
       && r.x.val() == val.s[k]
     {
-      var ino := get_ino(k);
+      var ino := get_ino(txn, k);
       if ino as uint64 == 0 {
         return None;
       }
-      var name := get_name(k);
+      var name := get_name(txn, k);
       NullTerminatePrefix(name);
       decode_encode(val.s[k].name);
       return Some(MemDirEnt(name, ino));
     }
 
-    method is_used(k: uint64) returns (p:bool)
-      requires Valid()
-      requires dir_off?(k)
+    method is_used(txn: Txn, k: uint64) returns (p:bool)
+      modifies file
+      requires Valid() ensures Valid()
+      requires has_jrnl(txn)
+      requires k as nat < |val.s|
       ensures p == val.s[k].used()
     {
-      var ino := get_ino(k);
+      var ino := get_ino(txn, k);
       p := ino as uint64 != 0;
     }
 
-    method is_name(k: uint64, needle: Bytes) returns (r:Option<Ino>)
-      requires Valid()
-      requires dir_off?(k)
+    method is_name(txn: Txn, k: uint64, needle: Bytes) returns (r:Option<Ino>)
+      modifies file
+      requires Valid() ensures Valid()
+      requires has_jrnl(txn)
+      requires k as nat < |val.s|
       requires needle.Valid()
       requires is_pathc(needle.data)
       ensures r.None? ==> !(val.s[k].used() && val.s[k].name == needle.data)
       ensures r.Some? ==> val.s[k].used() && val.s[k].name == needle.data && val.s[k].ino == r.x
     {
-      var ino := get_ino(k);
+      var ino := get_ino(txn, k);
       if ino as uint64 == 0 {
         return None;
       }
-      var name := get_name(k);
+      var name := get_name(txn, k);
       assert decode_null_terminated(name.data) == val.s[k].name by {
         decode_encode(val.s[k].name);
       }
@@ -316,36 +396,53 @@ module MemDirEntries
       }
     }
 
-    method findFree() returns (free_i: uint64)
+    method dirSize() returns (num: uint64)
       requires Valid()
+      ensures num as nat == |val.s|
+    {
+      var sz := file.size();
+      num := sz / 64;
+      reveal ValidCore();
+    }
+
+    method findFree(txn: Txn) returns (free_i: uint64)
+      modifies file
+      requires Valid() ensures Valid()
+      requires has_jrnl(txn)
       ensures free_i as nat == val.findFree()
     {
+      var num_ents := dirSize();
       var i: uint64 := 0;
-      while i < dir_sz_u64
-        invariant 0 <= i as nat <= dir_sz
+      while i < num_ents
+        invariant Valid()
+        invariant 0 <= i as nat <= |val.s|
         invariant forall k:nat | k < i as nat :: val.s[k].used()
       {
-        var p := is_used(i);
+        var p := is_used(txn, i);
         if !p {
           C.find_first_characterization(Dirents.is_unused, val.s, i as nat);
           return i;
         }
         i := i + 1;
       }
-      C.find_first_characterization(Dirents.is_unused, val.s, dir_sz);
-      return dir_sz_u64;
+      C.find_first_characterization(Dirents.is_unused, val.s, |val.s|);
+      return num_ents;
     }
 
-    method isEmpty() returns (p:bool)
-      requires Valid()
+    method isEmpty(txn: Txn) returns (p:bool)
+      modifies file
+      requires Valid() ensures Valid()
+      requires has_jrnl(txn)
       ensures p == (dir() == map[])
     {
+      var num_ents := dirSize();
       var i: uint64 := 0;
-      while i < dir_sz_u64
-        invariant 0 <= i as nat <= dir_sz
+      while i < num_ents
+        invariant Valid()
+        invariant 0 <= i as nat <= |val.s|
         invariant forall k:nat | k < i as nat :: !val.s[k].used()
       {
-        var p := is_used(i);
+        var p := is_used(txn, i);
         if p {
           seq_to_dir_present(val.s, i as nat);
           return false;
@@ -356,10 +453,12 @@ module MemDirEntries
       return true;
     }
 
-    method findName(name: Bytes) returns (r: Option<(uint64, Ino)>)
-      requires Valid()
+    method findName(txn: Txn, name: Bytes) returns (r: Option<(uint64, Ino)>)
+      modifies file
+      requires Valid() ensures Valid()
+      requires has_jrnl(txn)
       requires is_pathc(name.data)
-      ensures r.None? ==> name.data !in val.dir && val.findName(name.data) == dir_sz
+      ensures r.None? ==> name.data !in val.dir && val.findName(name.data) == |val.s|
       ensures r.Some? ==>
       && name.data in val.dir
       && dir_off?(r.x.0)
@@ -367,12 +466,14 @@ module MemDirEntries
       && val.dir[name.data] == r.x.1
     {
       ghost var p: PathComp := name.data;
+      var num_ents := dirSize();
       var i: uint64 := 0;
-      while i < dir_sz_u64
-        invariant 0 <= i as nat <= dir_sz
+      while i < num_ents
+        invariant Valid();
+        invariant 0 <= i as nat <= |val.s|
         invariant forall k:nat | k < i as nat :: !(val.s[k].used() && val.s[k].name == p)
       {
-        var ino := is_name(i, name);
+        var ino := is_name(txn, i, name);
         if ino.Some? {
           C.find_first_characterization(preDirents.findName_pred(p), val.s, i as nat);
           assert val.findName(p) == i as nat;
@@ -381,22 +482,26 @@ module MemDirEntries
         }
         i := i + 1;
       }
-      C.find_first_characterization(preDirents.findName_pred(p), val.s, dir_sz);
+      C.find_first_characterization(preDirents.findName_pred(p), val.s, |val.s|);
       val.findName_not_found(p);
       return None;
     }
 
-    method usedDents() returns (dents: seq<MemDirEnt>)
-      requires Valid()
+    method usedDents(txn: Txn) returns (dents: seq<MemDirEnt>)
+      modifies file
+      requires Valid() ensures Valid()
+      requires has_jrnl(txn)
       ensures mem_seq_valid(dents)
       ensures fresh(mem_dirs_repr(dents))
       ensures seq_to_dir(mem_seq_val(dents)) == val.dir
       ensures |dents| == |val.dir|
     {
       dents := [];
+      var num_ents := dirSize();
       var i: uint64 := 0;
-      while i < dir_sz_u64
-        invariant 0 <= i as nat <= dir_sz
+      while i < num_ents
+        invariant Valid()
+        invariant 0 <= i as nat <= |val.s|
         invariant |dents| <= i as nat
         invariant mem_seq_valid(dents)
         invariant fresh(mem_dirs_repr(dents))
@@ -404,7 +509,7 @@ module MemDirEntries
       {
         assert val.s[..i+1] == val.s[..i] + [val.s[i]];
         used_dirents_app(val.s[..i], [val.s[i]]);
-        var e := get_dirent(i);
+        var e := get_dirent(txn, i);
         if e.Some? {
           assert val.s[i].used();
           mem_dirs_repr_app(dents, [e.x]);
@@ -424,14 +529,14 @@ module MemDirEntries
         i := i + 1;
       }
 
-      assert val.s[..dir_sz] == val.s;
+      assert val.s[..|val.s|] == val.s;
       used_dirents_dir(val.s);
       used_dirents_size(val.s);
     }
 
     static method write_ent(bs: Bytes, k: uint64, ghost v: DirEnt, name: Bytes, ino: Ino)
       modifies bs
-      requires dir_off?(k)
+      requires k as nat < 64
       requires |bs.data| == 4096
       requires name.data == encode_pathc(v.name) && v.ino == ino
       ensures |v.enc()| == dirent_sz
@@ -442,36 +547,42 @@ module MemDirEntries
       IntEncoding.UInt64Put(ino, k*dirent_sz_u64 + path_len_u64, bs);
     }
 
-    method insert_ent(k: uint64, e: MemDirEnt)
-      modifies Repr, e.name
-      requires Valid() ensures Valid()
+    method {:verify false} insert_ent(txn: Txn, k: uint64, e: MemDirEnt)
+      returns (ok:bool)
+      modifies Repr(), e.name
+      requires Valid() ensures ok ==> Valid()
+      requires has_jrnl(txn)
       requires e.Valid() && e.used()
       requires dir_off?(k) && k as nat == val.findFree()
       requires val.findName(e.val().name) >= dir_sz
-      ensures val.dir == old(val.dir[e.val().name := e.val().ino])
+      ensures ok ==> val.dir == old(val.dir[e.val().name := e.val().ino])
     {
       reveal ValidCore();
       ghost var v := e.val();
       v.enc_len();
       val.insert_ent_dir(v);
-      val := seq_data_splice_one(bs.data, val, k as nat, v);
+      val := seq_data_splice_one(file.contents(), val, k as nat, v);
       // modify in place to re-use space
       PadPathc(e.name);
       var padded_name := e.name;
-      write_ent(this.bs, k, v, padded_name, e.ino);
+      loadDirOff(txn, k);
+      write_ent(file.bs, k % 64, v, padded_name, e.ino);
+      ok := file.writeback(txn);
     }
 
-    method deleteAt(k: uint64)
-      modifies Repr
-      requires Valid() ensures Valid()
+    method {:verify false} deleteAt(txn: Txn, k: uint64)
+      returns (ok: bool)
+      modifies Repr()
+      requires Valid() ensures ok ==> Valid()
       requires dir_off?(k) && val.s[k].used()
-      ensures val.dir == old(map_delete(val.dir, val.s[k].name))
+      ensures ok ==> val.dir == old(map_delete(val.dir, val.s[k].name))
     {
       reveal ValidCore();
       var old_name := val.s[k].name;
-      val := seq_data_splice_ino(bs.data, val, k as nat, 0 as Ino);
-      IntEncoding.UInt64Put(0, k*dirent_sz_u64 + path_len_u64, bs);
+      val := seq_data_splice_ino(file.contents(), val, k as nat, 0 as Ino);
+      IntEncoding.UInt64Put(0, (k%64)*dirent_sz_u64 + path_len_u64, file.bs);
       seq_to_dir_delete(old(val.s), k as nat, old_name);
+      ok := file.writeback(txn);
     }
   }
 }
